Updated Values with new Integers Int64 shift mask

lib/Integers.v
@@ -4683,12 +4683,12 @@ Proof.
   generalize (Int.unsigned_range_2 y). intros. lia.
 Qed.
 
-Definition shift_mask_long (v : int) : int := Int64.and v (Int64.repr 63).
+Definition shift_mask_long (v : Int.int) : Int.int := Int.and v (Int.repr 63).
 
 Theorem sem_mask_ident_int:
-forall v : int,
+forall v : Int.int,
 (*Int.ltu v Int64.iwordsize' = true -> val_shift_lng_mask v = v.*)
-(Int64.unsigned v) < Int64.zwordsize -> shift_mask_long v = v.
+(Int.unsigned v) < Int64.zwordsize -> shift_mask_long v = v.
 Proof. Admitted.
 
 End Int64.
