common/Values.v
@@ -724,9 +724,11 @@ Definition xorl (v1 v2: val): val :=
   | _, _ => Vundef
   end.
 
+Check Int64.shl'.
+
 Definition shll (v1 v2: val): val :=
   match v1, v2 with
-  | Vlong n1, Vint n2 => Vlong(Int64.shl' n1 (val_shift_lng_mask n2))
+  | Vlong n1, Vint n2 => Vlong(Int64.shl' n1 (Int64.shift_mask_long n2))
   | _, _ => Vundef
   end.
 
